# ECON2125/4021/8013 <br> Lecture 21 

John Stachurski

Semester 1, 2015

## Application: A Planning Problem

A firm

- owns stock $s_{t}$ of a natural resouce (e.g., oil)
- supplies $q_{t}$ at time $t$ and gets current profit $\pi\left(q_{t}\right)$

- stock next period is $s_{t+1}=s_{t}-q_{t}$

Suppose that $t=0$, current stock is $s_{0}$
Given supply sequence $\left\{q_{t}\right\}_{t=0}^{\infty}$, net present value of profits flow is

$$
\mathrm{NPV}=\sum_{t=0}^{\infty} \beta^{t} \pi\left(q_{t}\right) \quad \text { where } \quad \beta:=\frac{1}{1+r}
$$

Assume the resource is nonrenewable, so

$$
\text { sequence }\left\{q_{t}\right\} \text { feasible } \Longleftrightarrow \sum_{t=0}^{\infty} q_{t} \leq s_{0}
$$

Suppose that

- $s_{t}$ and $q_{t}$ take integer values
- $\pi(q)=q^{\alpha}$ for some $\alpha \in(0,1)$


Figure: Present value of different $\left\{q_{t}\right\}$ sequences $(\alpha=0.5, r=0.05)$

Assume that the firm chooses $\left\{q_{t}\right\}$ to maximize NPV
Let $v^{*}(s)$ be the NPV corresponding to

- current stock $s_{0}$ equal to $s$
- an optimal supply sequence choice given $s=s_{0}$

$$
v^{*}(s)=\sup \left\{\sum_{t=0}^{\infty} \beta^{t} \pi\left(q_{t}\right): \sum_{t=0}^{\infty} q_{t} \leq s\right\}
$$

Thus $v^{*}(s)$ is the "market value of the firm with current stock $s$ "
How to compute $v^{*}(s)$ for all $s \leq N=$ : some max level of stock?

It turns out that $v^{*}$ satisfies the equation

$$
v^{*}(s)=\max _{0 \leq q \leq s}\left\{\pi(q)+\beta v^{*}(s-q)\right\} \quad(s=0, \ldots, N)
$$

Intuition: Max value attained if current $q$ chosen to trade off

- current profits $\pi(q)$
- depletion of stock to $s-q$ weighted by future value

Proof: Omitted - see Bellman's principle of optimality
More intuition / examples of these kinds of recursions coming later
Remark: We're restricting $q$ to be an integer for simplicity

Let $\mathbf{v}=(v(0), \ldots, v(N))$ be any vector in $\mathbb{R}^{N+1}$
Consider creating a new vector $\hat{\mathbf{v}} \in \mathbb{R}^{N+1}$ from $\mathbf{v}$ via

$$
\hat{v}(s)=\max _{0 \leq q \leq s}\{\pi(q)+\beta v(s-q)\} \quad(s=0, \ldots, N)
$$

- $\hat{v}(0)=\max _{0 \leq q \leq 0}\{\pi(q)+\beta v(0-q)\}=\pi(0)+\beta v(0)$
- $\hat{v}(1)=\max _{0 \leq q \leq 1}\{\pi(q)+\beta v(1-q)\}=\cdots$


Figure : Creating $\hat{\mathbf{v}}$ from given $\mathbf{v}$

We've specified a rule that creates a new vector $\hat{\mathbf{v}}$ from any existing vector $\mathbf{v}$

We can think of this operation $\mathbf{v} \mapsto \hat{\mathbf{v}}$ as a mapping

Let $T$ be the mapping defined in this way
That is, $\hat{\mathbf{v}}=T \mathbf{v}$ where

$$
T v(s)=\max _{0 \leq q \leq s}\{\pi(q)+\beta v(s-q)\} \quad(s=0,1, \ldots, N)
$$

$T$ is a well-defined mapping from $\mathbb{R}^{N+1} \rightarrow \mathbb{R}^{N+1}$

Recall that

$$
v^{*}(s)=\max _{0 \leq q \leq s}\left\{\pi(q)+\beta v^{*}(s-q)\right\}
$$

and that $T: \mathbb{R}^{N+1} \rightarrow \mathbb{R}^{N+1}$ maps $\mathbf{v}$ to $\hat{\mathbf{v}}$ by

$$
T v(s)=\max _{0 \leq q \leq s}\{\pi(q)+\beta v(s-q)\}
$$

It follows that

$$
T v^{*}(s)=\max _{0 \leq q \leq s}\left\{\pi(q)+\beta v^{*}(s-q)\right\}=v^{*}(s)
$$

That is, $T \mathbf{v}^{*}=\mathbf{v}^{*}$
Thus, solving for $\mathbf{v}^{*}$ is the same as finding a fixed point of $T$

Claim: $T$ is a contraction on $\mathbb{R}^{N+1}$ with $p$-norm $\|\cdot\|_{\infty}$
Proof: Pick any $\mathbf{v}, \mathbf{w}$ in $\mathbb{R}^{N+1}$ and any $s$ in $0,1, \ldots, N$
By definition,

$$
\begin{aligned}
& |\operatorname{Tv}(s)-\operatorname{Tw}(s)|= \\
& \quad\left|\max _{0 \leq q \leq s}\{\pi(q)+\beta v(s-q)\}-\max _{0 \leq q \leq s}\{\pi(q)+\beta w(s-q)\}\right|
\end{aligned}
$$

Recall now the rule

$$
\left|\sup _{x \in A} f(x)-\sup _{x \in A} g(x)\right| \leq \sup _{x \in A}|f(x)-g(x)|
$$

Hence

$$
\begin{aligned}
|T v(s)-T w(s)| & \leq \max _{0 \leq q \leq s}|\pi(q)+\beta v(s-q)-(\pi(q)+\beta w(s-q))| \\
& =\beta \max _{0 \leq q \leq s}|v(s-q)-w(s-q)| \\
& \leq \beta \max _{0 \leq u \leq N}|v(u)-w(u)| \\
& =\beta\|\mathbf{v}-\mathbf{w}\|_{\infty}
\end{aligned}
$$

Since the last term is an upper bound on $|T v(s)-T w(s)|$, we have

$$
\|T \mathbf{v}-T \mathbf{w}\|_{\infty} \leq \beta\|\mathbf{v}-\mathbf{w}\|_{\infty}
$$

What we know so far

- $T$ has a unique fixed point in $\mathbb{R}^{N+1}$
- that fixed point is $\mathbf{v}^{*}$, the object we want to compute
- If $\mathbf{v}$ is any point in $\mathbb{R}^{N+1}$, then $T^{k} \mathbf{v} \rightarrow \mathbf{v}^{*}$

So let's pick $\mathbf{v}$ and iterate with $T$
In practice we

1. Iterate until $\left\|T^{k} \mathbf{v}-T^{k+1} \mathbf{v}\right\|_{\infty}<\epsilon:=$ small error tolerance
2. Take the final $T^{k} \mathbf{v}$ as approximate solution for $\mathbf{v}^{*}$


Figure : The sequence $\mathbf{v}, T \mathbf{v}, T^{2} \mathbf{v}, \ldots$ and limit


Figure: Iterates with alternative initial condition

## Comparative Statics

Now we know how to compute a solution $\mathbf{v}^{*}$ for each set of parameters

Typical next step: look at the properties of the solution
Example. How is the value of the firm affected by $r$ ?
Intuitively, higher interest rate decreases net present value Let's

- compute approximate $\mathbf{v}^{*}$ associated with different $r$
- see whether they do go down as $r$ goes up


Figure: The vector $\mathbf{v}^{*}$ computed at different values of $r$

## New Topic

## DYNAMICS

## Dynamics

Dynamics are essential to almost all areas of economics and finance

Why? Because the future matters for the present:

- Can't price an asset today without considering what it could be sold for tomorrow
- Can't analyze viability of a pension system without considering future time paths for income, savings, etc.
- Central banks can't choose interest rates without considering future inflation, unemployment and output


## Introductory Example: Solow-Swan

We start with a simple example: Solow-Swan growth

1. Agents save some of their current income
2. Those savings are used to increase capital stock
3. Capital is combined with labour to produce output
4. Output is income (divided out as wages, rent on capital)
5. Return to step 1

What happens to output / capital / etc. over time?

In the model, output in each period is

$$
Y_{t}=F\left(K_{t}, L_{t}\right) \quad(t=0,1,2, \ldots)
$$

Here

- $K_{t}=$ capital
- $L_{t}=$ labor
- $Y_{t}=$ output
- $F$ is the aggregate production function
$F$ assumed to be homogeneous of degree one (HD1), meaning

$$
F(\lambda K, \lambda L)=\lambda F(K, L) \quad \text { for all } \lambda \geq 0
$$

Examples.

Cobb-Douglas:

$$
F(K, L)=A K^{\alpha} L^{1-\alpha}
$$

CES:

$$
F(K, L)=\gamma\left\{\alpha K^{\rho}+(1-\alpha) L^{\rho}\right\}^{1 / \rho}
$$

Closed economy: current domestic investment $=$ aggregate domestic savings

The savings rate is a positive constant $s$, so

$$
\text { investment }=\text { savings }=s Y_{t}=s F\left(K_{t}, L_{t}\right)
$$

Depreciation means that 1 unit of capital today becomes $1-\delta$ units next period

Thus, capital stock evolves according to

$$
K_{t+1}=s F\left(K_{t}, L_{t}\right)+(1-\delta) K_{t}
$$

We simplify $K_{t+1}=s F\left(K_{t}, L_{t}\right)+(1-\delta) K_{t}$ as follows

Assume that $L_{t}=$ some constant $L$
Now set $k_{t}:=K_{t} / L$ and use HD1 to get the per capita law of motion

$$
\begin{aligned}
k_{t+1} & =s \frac{F\left(K_{t}, L\right)}{L}+(1-\delta) k_{t} \\
& =s F\left(k_{t}, 1\right)+(1-\delta) k_{t}
\end{aligned}
$$

Setting $f(k):=F(k, 1)$ to simplify notation, final expression is

$$
k_{t+1}=s f\left(k_{t}\right)+(1-\delta) k_{t}
$$

In summary, we can write

$$
k_{t+1}=g\left(k_{t}\right) \quad \text { where } \quad g(k):=s f(k)+(1-\delta) k
$$

This kind of equation is called a difference equation
In this case, scalar and nonlinear
Main question: what are the implied properties of $\left\{k_{t}\right\}$ ?

More generally, given

- difference equation $x_{t+1}=g\left(x_{t}\right)$
- initial condition $x_{0}$,
what are the properties of $\left\{x_{t}\right\}$ ?


## 45 Degree Diagrams

A method for tracing out dynamics graphically
Useful for analyzing one dimensional dynamic systems
Equally helpful for both linear and nonlinear systems
Let's look at some examples, starting with the difference equation

$$
x_{t+1}=g\left(x_{t}\right) \quad \text { when } \quad g(x)=2+0.5 x
$$

We want to be able to take any $x_{0}$ and map out the sequence

$$
x_{0}, \quad x_{1}=g\left(x_{0}\right), \quad x_{2}=g\left(x_{1}\right), \quad \ldots
$$

- g - 45


Figure: $g(x)=2+0.5 x$ with $x_{0}=0.4$


Figure: $g(x)=2+0.5 x$ with $x_{0}=1.5$


Figure: $g(x)=2+0.5 x$ with $x_{0}=5.8$

- g - 45


Figure: $g(x)=1+1.2 x$ with $x_{0}=0.4$

- g - 45


Figure : $g(x)=2.125 /\left(1+x^{-4}\right)$ with $x_{0}=0.85$


Figure: $g(x)=2.125 /\left(1+x^{-4}\right)$ with $x_{0}=1.1$

## Let's compare

- 45 degree diagrams
- corresponding time series plots
- g - 45


Figure: $g(x)=2+0.5 x$ with $x_{0}=0.4$


Figure: $g(x)=2+0.5 x$ with $x_{0}=0.4$

- g - 45


Figure: $g(x)=1+1.2 x$ with $x_{0}=0.4$


Figure : $g(x)=1+1.2 x$ with $x_{0}=0.4$


Figure : $g(x)=2.125 /\left(1+x^{-4}\right)$ and $g(0)=0$ with $x_{0}=0.85$


Figure : $g(x)=2.125 /\left(1+x^{-4}\right)$ and $g(0)=0$ with $x_{0}=0.85$


Figure : $g(x)=2.125 /\left(1+x^{-4}\right)$ and $g(0)=0$ with $x_{0}=1.1$


Figure : $g(x)=2.125 /\left(1+x^{-4}\right)$ and $g(0)=0$ with $x_{0}=1.1$

## Back to Solow-Swan

Let's return to the model

$$
k_{t+1}=g\left(k_{t}\right) \quad \text { where } \quad g(k):=s f(k)+(1-\delta) k
$$

Let's assume that

- $f(k)=A k^{\alpha}$ where $A=1$ and $\alpha=0.6$
- $s=0.3$ and $\delta=0.1$

The dynamics can be seen graphically


Figure: Solow-Swan dynamics, low initial capital


Figure: Solow-Swan dynamics, low initial capital


Figure: Solow-Swan dynamics, high initial capital


Figure : Solow-Swan dynamics, high initial capital

Graphical analysis of the model suggests that

- $k_{t}$ increases over time if $k_{0}$ is small
- $k_{t}$ decreases over time if $k_{0}$ is large
- $k_{t}$ converges to the same point regardless of $k_{0}$

To go further with our analysis we need some definitions and results...

